Java/src/Logic/ProtocolLogic.v
@@ -1,11 +1,11 @@
 Require Import Rel Open ILogic ILInsts BILogic BILInsts IBILogic SepAlg SepAlgMap
                UUSepAlg SepAlgInsts OpenILogic Pure ILEmbed PureInsts Subst Stack.
 Require Import Maps MapInterface MapFacts.
-Require Import Lang Traces ST AssertionLogic SpecLogic Util Program.
+Require Import Lang ST AssertionLogic SpecLogic Util Program.
 
-Definition PM := Map [protocol, @open var _ ST].
+Definition PM := Map [protocol, ST].
 
-Definition psasn := PM -> sasn.
+Definition psasn := PM -> STs -> sasn.
 
 Local Transparent ILPre_Ops.
 Local Transparent ILFun_Ops.
@@ -13,7 +13,7 @@ Local Transparent BILPre_Ops.
 Local Transparent BILFun_Ops.
 
 Program Definition psasn_subst (P : psasn) (sub : subst) : psasn := 
-  fun PM s => mk_tasn (fun trs => mk_asn (fun Pr k h => P PM (stack_subst s sub) trs Pr k h) _ _ _) _.
+  fun PM STs s => mk_asn (fun Pr k h => P PM STs (stack_subst s sub) Pr k h) _ _ _.
 Next Obligation.
   solve_model H.
   congruence.
@@ -26,24 +26,26 @@ Next Obligation.
   solve_model H0.
   congruence.
 Defined.
-Next Obligation.
-  solve_model H0.
-  congruence.
-Defined.
 
-Program Definition ST_exists (p : protocol) (T : open ST) : psasn :=
-  fun PM s => mk_tasn (fun trs => mk_asn (fun P k h =>
+Program Definition ST_exists (p : protocol) (T : ST) : psasn :=
+  fun PM STs s => mk_asn (fun P k h =>
     MapsTo p T PM
-  ) _ _ _) _.
+  ) _ _ _.
 
-Program Definition all_traces_eq (t : trace) : psasn :=
-  fun PM s => mk_tasn (fun trs => mk_asn (fun P k h =>
-    forall c, In c trs -> MapsTo c t trs
-  ) _ _ _) _.
-Next Obligation.
-  rewrite <- H in *.
-  apply H0; assumption.
-Defined.
+Program Definition has_ST (v : var) (T : ST) : psasn :=
+  fun PM STs s => mk_asn (fun P k h =>
+    MapsTo (val_to_stptr (s v)) T STs
+  ) _ _ _.
+
+Program Definition has_subst_ST (x z y : var) (T : ST) : psasn :=
+  fun PM STs s => mk_asn (fun P k h =>
+    MapsTo (val_to_stptr (s x)) (subst_ST z (s y) T) STs
+  ) _ _ _.
+
+Program Definition all_STs (T : ST) : psasn :=
+  fun PM STs s => mk_asn (fun P k h =>
+    forall c, In c STs -> MapsTo c T STs
+  ) _ _ _.
 
 Local Existing Instance ILPre_Ops.
 Local Existing Instance ILPre_ILogic.
@@ -95,3 +97,105 @@ Instance EmbedPSasnSpec   : Embed spec psasn   := _.
 
 Instance EmbedPSasnSasnOp : EmbedOp sasn psasn := _. 
 Instance EmbedPSasnSasn   : Embed sasn psasn := _.
+
+Module IsMarshallable.
+  Require Import Heap Relations RelationPairs.
+  Import Marshall.
+  
+  Program Definition isMarshallable (v : var) (P : psasn) : psasn :=
+  	fun PM STs s => mk_asn (fun Pr k h =>
+    	forall h' Pr' k' (Hk: k' <= k) (HPr: Prog_wf_sub Pr Pr'), P PM STs s Pr' k' h' -> marshall (s v) h h'
+  	) _ _ _.
+  Next Obligation.
+    eapply H with (k' := k').
+    omega.
+    apply HPr.
+    solve_model H0.
+  Defined.
+  Next Obligation.
+    eapply H0. 
+    apply Hk.
+    transitivity P'; eassumption.
+    solve_model H1.
+  Defined.
+  Next Obligation.
+    eapply marshall_from_smaller; [eassumption |].
+    eapply H0; eassumption.
+  Defined.
+
+  Local Transparent EmbedILFunDropOp.
+  Local Transparent EmbedILFunOp.
+  Local Transparent EmbedAsnPropOp.
+  Local Transparent RelCompFun.
+  
+  Local Existing Instance MapSepAlgOps.
+  Local Existing Instance MapSepAlg.
+  Local Existing Instance MapEquiv.
+  Local Existing Instance EquivPreorder.
+  Local Existing Instance UUMapSepAlg.
+  Local Existing Instance SepAlgOps_prod.
+  Local Existing Instance SepAlg_prod.
+  Local Existing Instance UUSepAlg_prod.
+
+  Lemma pointsto_isMarshallable (p : var) (ptr : ptr) (f : field) (v : val) :
+    forall PM STs (s:stack) Pr k h  
+    (Href: s p = (vptr ptr)) (Hpointsto: (pointsto (vptr ptr) f v) Pr k h), 
+    (isMarshallable p (embed (pointsto (vptr ptr) f v))) PM STs s Pr k h
+    .
+  Proof.
+    admit.
+    (*
+    intros. 
+    simpl in Hpointsto.
+    
+    simpl. intros.
+    destruct Hpointsto as [Hnotnull Hpointsto].
+    destruct H as [H'notnull H'pointsto].
+    unfold subheap in H'pointsto.
+    destruct H'pointsto as [h'' H'pointsto].
+    
+    assert (h' = heap_add_ptr (mkheap h'' (get_heap_arr h')) ptr f v). admit.
+    rewrite H.
+    constructor. apply Href.
+    unfold subheap in Hpointsto; destruct Hpointsto as [? Hpointsto].
+    eapply sa_mul_mapstoL in Hpointsto.
+    apply Hpointsto.
+    apply add_1. reflexivity.
+    
+      unfold subheap in H'pointsto.
+      destruct H'pointsto as [h'' H'pointsto].
+      exists (mkheap h'' (get_heap_arr h')).
+      
+      split. intro key. unfold heap_add_ptr, mkheap, get_heap_arr; simpl.
+      simpl in H'pointsto.
+      specialize (H'pointsto key).
+      remember (find key (get_heap_ptr h')).
+      simpl in Heqo; rewrite <- Heqo in H'pointsto.
+      destruct o; unfold get_heap_ptr in Heqo; rewrite <- Heqo.
+      destruct H'pointsto as [[H'pointsto _] | [H'pointsto _]].
+      destruct (eq_dec key (ptr, f)).
+      rewrite H in H'pointsto.
+      apply map_mapsto_add_eq in H'pointsto; rewrite H'pointsto.
+      rewrite add_eq_o; [| auto]. reflexivity.
+      apply add_neq_mapsto_iff in H'pointsto; [| symmetry; auto].
+      apply empty_mapsto_iff in H'mapsto. inversion H'mapsto.
+      
+      apply find_mapsto_iff in H'pointsto. rewrite H'mapsto. reflexivity.
+      apply add_1; auto.
+      rewrite add_neq_o; [| symmetry; auto].
+      unfold sa_mul in H'pointsto. simpl in H'pointsto.
+      eapply sa_mul_mapstoR in H'pointsto.
+      destruct H'pointsto as [[H'mapsto _] | [H'mapsto _] ].
+      
+      apply add_neq_mapsto_iff in H'mapsto. apply empty_mapsto_iff in H'mapsto. inversion H'mapsto.
+      symmetry; apply H.
+      
+      SearchAbout MapsTo empty.
+      
+      
+    apply marshall_ptr.*)
+      Admitted.
+
+End IsMarshallable.
+
+
