Java/src/Semantics/SemCmd.v
@@ -1,7 +1,7 @@
 Require Import SepAlg OpenILogic SepAlgMap.
 Require Import MapInterface MapFacts.
 Require Import ILInsts ILogic ILEmbed Open Subst Stack.
-Require Import Program SpecLogic Heap ProtocolLogic Lang Traces.
+Require Import Program SpecLogic Heap ProtocolLogic Lang ST.
 
 Import SepAlgNotations.
 
@@ -11,26 +11,26 @@ Set Maximal Implicit Insertion.
 
 Section Commands.
 
-  Definition semCmdType := Prog_wf -> PM -> nat -> stack -> heap -> traces -> option (stack * (heap * traces)) -> Prop.
-  Definition safe (c : semCmdType) Pr PM n s h t := ~(c Pr PM n s h t None).
+  Definition semCmdType := Prog_wf -> PM -> nat -> stack -> heap -> STs -> option (stack * (heap * STs)) -> Prop.
+  Definition safe (c : semCmdType) Pr PM n s h STs := ~(c Pr PM n s h STs None).
   Definition frame_property (c : semCmdType) :=
-    forall Pr PM s s' (big big' frame h : heap) n t t'
+    forall Pr PM s s' (big big' frame h : heap) n STs STs'
       (HFrame : sa_mul h frame big)
-      (HSafe  : forall m, m <= n -> safe c Pr PM m s h t)
-      (HSem   : c Pr PM n s big t (Some (s', (big', t')))),
-      exists h', sa_mul h' frame big' /\ c Pr PM n s h t (Some (s', (h', t'))).
+      (HSafe  : forall m, m <= n -> safe c Pr PM m s h STs)
+      (HSem   : c Pr PM n s big STs (Some (s', (big', STs')))),
+      exists h', sa_mul h' frame big' /\ c Pr PM n s h STs (Some (s', (h', STs'))).
 
   Record semCmd := {
-    cmd_rel   :> Prog_wf -> PM -> nat -> stack -> heap -> traces -> option (stack * (heap * traces)) -> Prop;
+    cmd_rel   :> Prog_wf -> PM -> nat -> stack -> heap -> STs -> option (stack * (heap * STs)) -> Prop;
     cmd_zero  :  forall Pr PM s h t cfg, ~(cmd_rel Pr PM 0 s h t cfg);
     cmd_frame :  frame_property cmd_rel
   }.
 
   Definition not_modifies (c : semCmdType) x : Prop :=
-    forall Pr PM s s' h h' n t t' (HSem : c Pr PM n s h t (Some (s', (h', t')))),
+    forall Pr PM s s' h h' n STs STs' (HSem : c Pr PM n s h STs (Some (s', (h', STs')))),
       s x = s' x.
 
-  Lemma safe_zero : forall (c : semCmd) Pr PM s h t, safe c Pr PM 0 s h t.
+  Lemma safe_zero : forall (c : semCmd) Pr PM s h STs, safe c Pr PM 0 s h STs.
   Proof.
     intros; apply cmd_zero.
   Qed.
@@ -40,7 +40,7 @@ Section Commands.
   Implicit Arguments Build_semCmd [].
 
   Program Definition later_cmd (c : semCmd) : semCmd := Build_semCmd
-    (fun Pr PM n => match n return stack -> heap -> traces -> option (stack * (heap * traces)) -> Prop with
+    (fun Pr PM n => match n return stack -> heap -> STs -> option (stack * (heap * STs)) -> Prop with
                   | O => fun _ _ _ _ => False
                   | S n => c Pr PM n end) _ _.
   Next Obligation.
@@ -51,7 +51,7 @@ Section Commands.
   Qed.
 
   Inductive skip_sem : semCmdType :=
-  | s_ok : forall Pr PM s h t, skip_sem Pr PM 1 s h t (Some (s, (h, t))).
+  | s_ok : forall Pr PM s h STs, skip_sem Pr PM 1 s h STs (Some (s, (h, STs))).
   Program Definition skip_cmd := @Build_semCmd skip_sem _ _.
   Next Obligation.
     intros H. inversion H.
@@ -64,17 +64,17 @@ Section Commands.
 
   (* Seq *)
   Inductive seq_sem (c1 c2 : semCmd) : semCmdType :=
-  | seq_failL : forall Pr PM n s h t,
-      c1 Pr PM n s h t None ->
-      seq_sem c1 c2 Pr PM (S n) s h t None
-  | seq_failR : forall Pr PM n n' s s' h h' t t',
-      c1 Pr PM n s h t (Some (s', (h', t'))) ->
-      c2 Pr PM n' s' h' t' None ->
-      seq_sem c1 c2 Pr PM (S (n + n')) s h t None
-  | seq_ok    : forall Pr PM n n0 s s0 s1 h h0 h1 t t0 t1,
-      c1 Pr PM n  s  h  t  (Some (s0, (h0, t0))) ->
-      c2 Pr PM n0 s0 h0 t0 (Some (s1, (h1, t1))) ->
-      seq_sem c1 c2 Pr PM (S (n + n0)) s h t (Some (s1, (h1, t1))).
+  | seq_failL : forall Pr PM n s h STs,
+      c1 Pr PM n s h STs None ->
+      seq_sem c1 c2 Pr PM (S n) s h STs None
+  | seq_failR : forall Pr PM n n' s s' h h' STs STs',
+      c1 Pr PM n s h STs (Some (s', (h', STs'))) ->
+      c2 Pr PM n' s' h' STs' None ->
+      seq_sem c1 c2 Pr PM (S (n + n')) s h STs None
+  | seq_ok    : forall Pr PM n n0 s s0 s1 h h0 h1 STs STs0 STs1,
+      c1 Pr PM n  s  h  STs  (Some (s0, (h0, STs0))) ->
+      c2 Pr PM n0 s0 h0 STs0 (Some (s1, (h1, STs1))) ->
+      seq_sem c1 c2 Pr PM (S (n + n0)) s h STs (Some (s1, (h1, STs1))).
   Program Definition seq_cmd c1 c2 := @Build_semCmd (seq_sem c1 c2) _ _.
   Next Obligation.
     intros H; inversion H.
@@ -90,18 +90,18 @@ Section Commands.
 
   (* Nondet *)
   Inductive nondet_sem (c1 c2 : semCmd) : semCmdType :=
-  | nondet_failL : forall Pr PM n s h t,
-      c1 Pr PM n s h t None ->
-      nondet_sem c1 c2 Pr PM (S n) s h t None
-  | nondet_okL   : forall Pr PM n s s' h h' t t',
-      c1 Pr PM n s h t (Some (s', (h', t'))) ->
-      nondet_sem c1 c2 Pr PM (S n) s h t (Some (s', (h', t')))
-  | nondet_failR : forall Pr PM n s h t,
-      c2 Pr PM n s h t None ->
-      nondet_sem c1 c2 Pr PM (S n) s h t None
-  | nondet_okR   : forall Pr PM n s s' h h' t t',
-      c2 Pr PM n s h t (Some (s', (h', t'))) ->
-      nondet_sem c1 c2 Pr PM (S n) s h t (Some (s', (h', t'))).
+  | nondet_failL : forall Pr PM n s h STs,
+      c1 Pr PM n s h STs None ->
+      nondet_sem c1 c2 Pr PM (S n) s h STs None
+  | nondet_okL   : forall Pr PM n s s' h h' STs STs',
+      c1 Pr PM n s h STs (Some (s', (h', STs'))) ->
+      nondet_sem c1 c2 Pr PM (S n) s h STs (Some (s', (h', STs')))
+  | nondet_failR : forall Pr PM n s h STs,
+      c2 Pr PM n s h STs None ->
+      nondet_sem c1 c2 Pr PM (S n) s h STs None
+  | nondet_okR   : forall Pr PM n s s' h h' STs STs',
+      c2 Pr PM n s h STs (Some (s', (h', STs'))) ->
+      nondet_sem c1 c2 Pr PM (S n) s h STs (Some (s', (h', STs'))).
   Program Definition nondet_cmd c1 c2 := @Build_semCmd (nondet_sem c1 c2) _ _.
   Next Obligation.
     intros H; inversion H.
@@ -117,26 +117,26 @@ Section Commands.
 
   (* Kleene star *)
   Inductive kleene_sem (c : semCmd) : semCmdType :=
-  | kleene_emp       : forall Pr PM s h t,
-      kleene_sem c Pr PM 1 s h t (Some (s, (h, t)))
-  | kleene_fail_one  : forall Pr PM n s h t,
-      c Pr PM n s h t None ->
-      kleene_sem c Pr PM (S n) s h t None
-  | kleene_fail_many : forall Pr PM n n0 s s0 h h0 t t0,
-      c Pr PM n s h t (Some (s0, (h0, t0))) ->
-      kleene_sem c Pr PM n0 s0 h0 t0 None ->
-      kleene_sem c Pr PM (S (n + n0)) s h t None
-  | kleene_step_ok   : forall Pr PM n n0 s s0 s1 h h0 h1 t t0 t1,
-      c Pr PM n s h t (Some (s0, (h0, t0))) ->
-      kleene_sem c Pr PM n0 s0 h0 t0 (Some (s1, (h1, t1))) ->
-      kleene_sem c Pr PM (S (n + n0)) s h t (Some (s1, (h1, t1))).
+  | kleene_emp       : forall Pr PM s h STs,
+      kleene_sem c Pr PM 1 s h STs (Some (s, (h, STs)))
+  | kleene_fail_one  : forall Pr PM n s h STs,
+      c Pr PM n s h STs None ->
+      kleene_sem c Pr PM (S n) s h STs None
+  | kleene_fail_many : forall Pr PM n n0 s s0 h h0 STs STs0,
+      c Pr PM n s h STs (Some (s0, (h0, STs0))) ->
+      kleene_sem c Pr PM n0 s0 h0 STs0 None ->
+      kleene_sem c Pr PM (S (n + n0)) s h STs None
+  | kleene_step_ok   : forall Pr PM n n0 s s0 s1 h h0 h1 STs STs0 STs1,
+      c Pr PM n s h STs (Some (s0, (h0, STs0))) ->
+      kleene_sem c Pr PM n0 s0 h0 STs0 (Some (s1, (h1, STs1))) ->
+      kleene_sem c Pr PM (S (n + n0)) s h STs (Some (s1, (h1, STs1))).
   Program Definition kleene_cmd c := @Build_semCmd (kleene_sem c) _ _.
   Next Obligation.
     intros H; inversion H.
   Qed.
   Next Obligation with eauto using kleene_sem.
     unfold frame_property; intros.
-    generalize dependent h; remember (Some (s', (big', t'))) as cfg; induction HSem;
+    generalize dependent h; remember (Some (s', (big', STs'))) as cfg; induction HSem;
       inversion Heqcfg; subst; intros; clear Heqcfg...
     edestruct (@cmd_frame c) as [h' [HFrame0 HSem0]]...
     + intros m HLe HFail; apply HSafe with (S m); [omega |]...
@@ -149,29 +149,29 @@ Section Commands.
      a check holds and loops otherwise, this way allowing to encode if/while
      using nondeterministic choice/Kleene star *)
   Inductive assume_sem (p : vlogic) : semCmdType :=
-  | assume_ok : forall Pr PM s h t, p s -> assume_sem p Pr PM 1 s h t (Some (s, (h, t))).
+  | assume_ok : forall Pr PM s h STs, p s -> assume_sem p Pr PM 1 s h STs (Some (s, (h, STs))).
   Program Definition assume_cmd P := @Build_semCmd (assume_sem P) _ _.
   Next Obligation.
     intros H; inversion H.
   Qed.
   Next Obligation.
     unfold frame_property; simpl; intros.
-    remember (Some (s', (big', t'))) as cfg; induction HSem.
+    remember (Some (s', (big', STs'))) as cfg; induction HSem.
     inversion Heqcfg; subst; eauto using assume_sem.
   Qed.
 
-  Lemma assume_inv Pr PM e n s s0 h h0 t t0 (HSem : assume_cmd e Pr PM n s h t (Some (s0, (h0, t0)))) : 
-      s = s0 /\ h = h0 /\ t = t0.
+  Lemma assume_inv Pr PM e n s s0 h h0 STs STs0 (HSem : assume_cmd e Pr PM n s h STs (Some (s0, (h0, STs0)))) : 
+      s = s0 /\ h = h0 /\ STs = STs0.
   Proof.  
-    intros; remember (Some (s0, (h0, t0))); induction HSem; subst;
+    intros; remember (Some (s0, (h0, STs0))); induction HSem; subst;
     try inversion Heqo; intuition.
   Qed.
 
   Inductive assert_sem (p : vlogic) : semCmdType :=
-  | assert_ok   : forall Pr PM s h t (HP : p s),
-    assert_sem p Pr PM 1 s h t (Some (s, (h, t)))
-  | assert_fail : forall Pr PM s h t (HNP : ~p s),
-    assert_sem p Pr PM 1 s h t None.
+  | assert_ok   : forall Pr PM s h STs (HP : p s),
+    assert_sem p Pr PM 1 s h STs (Some (s, (h, STs)))
+  | assert_fail : forall Pr PM s h STs (HNP : ~p s),
+    assert_sem p Pr PM 1 s h STs None.
   Program Definition assert_cmd p := @Build_semCmd (assert_sem p) _ _.
   Next Obligation.
     intros H; inversion H.
@@ -183,12 +183,12 @@ Section Commands.
 
   (* |= {p}c{q} *)
   Program Definition sem_triple (p q : psasn) (c : semCmd) : spec :=
-    mk_spec (fun P n => forall P' PM m k s h t, Prog_wf_sub P P' -> m <= n -> k <= m -> 
-                                           p PM s t P' m h ->
-      (safe c P' PM k s h t) /\
-      (forall t' h' s',  
-      	c P' PM k s h t (Some (s', (h', t'))) ->
-      		(q PM s' t' P' (m - k) h')
+    mk_spec (fun P n => forall P' PM m k s h STs, Prog_wf_sub P P' -> m <= n -> k <= m -> 
+                                           p PM STs s P' m h ->
+      (safe c P' PM k s h STs) /\
+      (forall STs' h' s',  
+      	c P' PM k s h STs (Some (s', (h', STs'))) ->
+      		(q PM STs' s' P' (m - k) h')
       		
       )
     ) _ _.
