Java/src/Semantics/SemCmdRules.v
@@ -1,7 +1,7 @@
 Require Import SemCmd ILogic BILogic ILInsts BILInsts. 
 Require Import OpenILogic Later ProtocolLogic AssertionLogic SpecLogic ILEmbed Open.
 Require Import Stack Subst Lang Util List.
-Require Import FunctionalExtensionality Traces.
+Require Import FunctionalExtensionality ST.
 
 Set Implicit Arguments.
 Unset Strict Implicit.
@@ -35,7 +35,7 @@ Section Rules.
     Qed.
 
     Definition not_modifies (c : semCmd) (x : var) : Prop :=
-      forall PP PM s s' h h' t t' n (HSem : c PP PM n s h t (Some (s', (h', t')))),
+      forall PP PM s s' h h' STs STs' n (HSem : c PP PM n s h STs (Some (s', (h', STs')))),
         s x = s' x.
         
     Lemma frame_rule : forall (P Q : psasn) (R : sasn) c (xs: list var)
@@ -46,27 +46,24 @@ Section Rules.
       intros.
       intros PP n HSpec PP' ? ? ? ? ? ? HPP' Hmn Hkm [h1 [h2 [HSub [HP HR]]]]; split.
       (* safety *)
-      { destruct (HSpec _ PM m k s h t HPP' Hmn Hkm) as [HS _]; [ | assumption].
+      { destruct (HSpec _ PM m k s h STs HPP' Hmn Hkm) as [HS _]; [ | assumption].
         solve_model HP. exists h2; apply HSub.
       }
       (* correctness *)
       intros ? ? ? HSem. 
-      destruct (@cmd_frame c PP' PM s s' h h' h2 h1 k t t') as [h'' [HBig Hc]]. 
+      destruct (@cmd_frame c PP' PM s s' h h' h2 h1 k STs STs') as [h'' [HBig Hc]]. 
       + assumption.
       + intros l Hle.
-        destruct (HSpec _ PM m l s h1 t HPP' Hmn) as [HS _]; [ omega | assumption |].
+        destruct (HSpec _ PM m l s h1 STs HPP' Hmn) as [HS _]; [ omega | assumption |].
         apply HS.
       + assumption.
-      + destruct (HSpec _ PM m k s h1 t HPP' Hmn Hkm) as [_ HC]. 
+      + destruct (HSpec _ PM m k s h1 STs HPP' Hmn Hkm) as [_ HC]. 
         * apply HP.
-        * specialize (HC t' h'' s' Hc).
+        * specialize (HC STs' h'' s' Hc).
           exists h'', h2, HBig. split; [assumption |].
           simpl. exists s. unfold apply_subst, id.
           simpl in HR; unfold id in HR.
           solve_model HR.
-          - unfold Rel.rel, MapInterface.Equal.
-            intros x.
-            admit (* fangel, tasn *).
           - apply functional_extensionality. intros x.
             unfold stack_subst, subst_fresh.
             destruct (in_dec Rel.dec_eq x xs) as [|HNotIn]; [reflexivity|].
@@ -81,9 +78,9 @@ Section Rules.
       G |-- {{P1 //\\ P2}} c {{Q1 //\\ Q2}}.
     Proof.
       intros n P HPP HG.
-      simpl. intros PM m k s h t HPP' Hm Hk [HP1 HP2]. split.
+      simpl. intros PM m k s h STs HPP' Hm Hk [HP1 HP2]. split.
       + eapply H1; eauto.
-      + intros t' h' s' Hsem.
+      + intros STs' h' s' Hsem.
         split; [eapply H1|eapply H2]; eauto.
     Qed.
 
@@ -93,28 +90,28 @@ Section Rules.
 
     Lemma skip_rule P : |-- {{P}}skip_cmd {{P}}.
     Proof.
-      intros PM n Pr HPP Pr' m k s h t _ Hmn Hkm HP; split.
+      intros PM n Pr HPP Pr' m k s h STs _ Hmn Hkm HP; split.
       + intros H; inversion H.
-      + intros t' h' s' HSem; inversion HSem; subst.
+      + intros STs' h' s' HSem; inversion HSem; subst.
         solve_model HP.
     Qed.
 
     Lemma seq_rule c1 c2 P Q R :
       ({{P}}c1{{Q}} //\\ {{Q}}c2{{R}}) |-- {{P}}seq_cmd c1 c2{{R}}.
     Proof.
-      intros Pr n [Hc1 Hc2] Pr' PM k m s h t HPP' Hmn Hkm HP; split.
+      intros Pr n [Hc1 Hc2] Pr' PM k m s h STs HPP' Hmn Hkm HP; split.
       + intros HFail; inversion HFail; subst; clear HFail.	
-        * destruct (Hc1 _ PM _ n0 s h t HPP' Hmn) as [HS _];
+        * destruct (Hc1 _ PM _ n0 s h STs HPP' Hmn) as [HS _];
           [omega | assumption | apply HS; assumption ].
-        * destruct (Hc1 _ PM _ n0 s h t HPP' Hmn) as [_ HC]; [omega | assumption |].
+        * destruct (Hc1 _ PM _ n0 s h STs HPP' Hmn) as [_ HC]; [omega | assumption |].
           specialize (HC _ _ _ H).
-          destruct (Hc2 _ PM (k - n0) n' s' h' t' HPP') as [HS _]; [omega | omega | |].
+          destruct (Hc2 _ PM (k - n0) n' s' h' STs' HPP') as [HS _]; [omega | omega | |].
           apply HC. 
           apply HS; exact H0.
-      + intros t' h' s' HSem; inversion HSem; subst; clear HSem.
-        destruct (Hc1 _ PM _ n0 s h t HPP' Hmn) as [_ HC1]; [omega | assumption |].
+      + intros STs' h' s' HSem; inversion HSem; subst; clear HSem.
+        destruct (Hc1 _ PM _ n0 s h STs HPP' Hmn) as [_ HC1]; [omega | assumption |].
         specialize (HC1 _ _ _ H7).
-        destruct (Hc2 _ PM (k - n0) n1 s1 h1 t1 HPP') as [_ HC2]; [omega | omega | |].
+        destruct (Hc2 _ PM (k - n0) n1 s1 h1 STs1 HPP') as [_ HC2]; [omega | omega | |].
         apply HC1.
         specialize (HC2 _ _ _ H9).
         solve_model HC2. 
@@ -123,17 +120,17 @@ Section Rules.
     Lemma nondet_rule c1 c2 P Q:
       ({{P}}c1{{Q}} //\\ {{P}}c2{{Q}}) |-- {{P}}nondet_cmd c1 c2{{Q}}.
     Proof.
-      intros n Pr [Hc1 Hc2] Pr' PM k m s h t HPP' Hmn Hkm HP; split.
+      intros n Pr [Hc1 Hc2] Pr' PM k m s h STs HPP' Hmn Hkm HP; split.
       + intros HFail; inversion HFail; subst; clear HFail.
-        * destruct (Hc1 _ PM _ n0 s h t HPP' Hmn) as [HS _];
+        * destruct (Hc1 _ PM _ n0 s h STs HPP' Hmn) as [HS _];
           [omega | assumption | apply HS; assumption].
-        * destruct (Hc2 _ PM _ n0 s h t HPP' Hmn) as [HS _];
+        * destruct (Hc2 _ PM _ n0 s h STs HPP' Hmn) as [HS _];
           [omega | assumption | apply HS; assumption].
-      + intros h1 s1 t1 HSem; inversion HSem; subst; clear HSem.
-        * destruct (Hc1 _ PM _ n0 s h t HPP' Hmn) as [_ HC]; [omega | assumption |].
+      + intros h1 s1 STs1 HSem; inversion HSem; subst; clear HSem.
+        * destruct (Hc1 _ PM _ n0 s h STs HPP' Hmn) as [_ HC]; [omega | assumption |].
           specialize (HC _ _ _ H6). 
           solve_model HC.
-        * destruct (Hc2 _ PM _ n0 s h t HPP' Hmn) as [_ HC]; [omega | assumption |].
+        * destruct (Hc2 _ PM _ n0 s h STs HPP' Hmn) as [_ HC]; [omega | assumption |].
           specialize (HC _ _ _ H6).
           solve_model HC.
     Qed.
@@ -141,21 +138,21 @@ Section Rules.
     Lemma kleene_rule c P:
       {{P}}c{{P}} |-- {{P}} kleene_cmd c {{P}}.
     Proof.
-      intros Pr n Hc Pr' PM m k s h t HPP' Hmn Hkm Hp; split.
+      intros Pr n Hc Pr' PM m k s h STs HPP' Hmn Hkm Hp; split.
       + intros HFail. generalize dependent m. remember None as cfg.
         induction HFail; intros; inversion Heqcfg; subst.
-        * destruct (Hc _ PM m n0 s h t HPP' Hmn) as [HS _];
+        * destruct (Hc _ PM m n0 s h STs HPP' Hmn) as [HS _];
           [omega | assumption | apply HS; assumption].
-        * destruct (Hc _ PM m n0 s h t HPP' Hmn) as [_ HC]; [omega | assumption |].
+        * destruct (Hc _ PM m n0 s h STs HPP' Hmn) as [_ HC]; [omega | assumption |].
           apply IHHFail with (m-n0); [assumption | reflexivity | omega | omega | ].
           specialize (HC _ _ _ H).
           solve_model HC.
-      + intros. remember (Some (s', (h', t'))) as cfg. generalize dependent m. 
+      + intros. remember (Some (s', (h', STs'))) as cfg. generalize dependent m. 
         induction H; inversion Heqcfg; subst; intros.
         * solve_model Hp.
-        * destruct (Hc _ PM m n0 s h t HPP' Hmn) as [_ HC]; [omega | assumption |].
+        * destruct (Hc _ PM m n0 s h STs HPP' Hmn) as [_ HC]; [omega | assumption |].
           specialize (HC _ _ _ H).
-          assert ((((P PM s') t' Pr0) ((m - n0) - n1)) h') as H2. 
+          assert ((((P PM STs' s') Pr0) ((m - n0) - n1)) h') as H2. 
             apply IHkleene_sem; try assumption; try omega. 
           solve_model H2.
     Qed.
@@ -163,9 +160,9 @@ Section Rules.
     Lemma assume_rule P (t : vlogic) :
       |-- {{P}} assume_cmd t {{t /\\ P}}.
     Proof.
-      intros n Pr Hc Pr' PM m k s h tr HPP' Hmn Hkm Hp; split.
+      intros n Pr Hc Pr' PM m k s h STs HPP' Hmn Hkm Hp; split.
       + intros HFail. inversion HFail.
-      + intros tr' h' s' H. remember (Some (s', (h', tr'))) as cfg; induction H.
+      + intros STs' h' s' H. remember (Some (s', (h', STs'))) as cfg; induction H.
         inversion Heqcfg; subst; intros.
         split; [assumption|]. solve_model Hp.
     Qed.
@@ -173,9 +170,9 @@ Section Rules.
     Lemma assert_rule (P : psasn) (p : vlogic) (HPe : P |-- embed p) :
       |-- {{P}} assert_cmd p {{P}}.
     Proof.
-      intros n Pr Hc Pr' PM m k s h t HPP' Hmn Hkm Hp; specialize (HPe _ _ _ _ _ _ Hp); split.
+      intros n Pr Hc Pr' PM m k s h STs HPP' Hmn Hkm Hp; specialize (HPe _ _ _ _ _ _ Hp); split.
       + intros HF; inversion HF; subst; auto.
-      + intros t' h' s' HSem; inversion HSem; subst.
+      + intros STs' h' s' HSem; inversion HSem; subst.
         solve_model Hp.
     Qed.
 
@@ -185,8 +182,8 @@ Section Rules.
     (Forall x, {{P x}} c {{q}}) -|- {{Exists x, P x}} c {{q}}.
   Proof.
   	split.
-  	+ intros n Pr Hp Pr' PM m k s h t HPP' Hmn Hkm [x Hxp]; specialize (Hp x); auto.
-  	+ intros n Pr Hp x Pr' PM m k s h t HPP' Hmn Hkm Hxp.
+  	+ intros n Pr Hp Pr' PM m k s h STs HPP' Hmn Hkm [x Hxp]; specialize (Hp x); auto.
+  	+ intros n Pr Hp x Pr' PM m k s h STs HPP' Hmn Hkm Hxp.
   	  apply Hp; try assumption. exists x; apply Hxp.
   Qed.
 
@@ -196,10 +193,10 @@ Section Rules.
     (SP -->> {{ P }} c {{ Q }}) -|- {{ SP /\\  P }} c {{ Q }}.
   Proof.
   	split.
-  	+ intros Pr n Hp Pr' PM m k s h t HPP' Hmn Hkm [HSP HP].
+  	+ intros Pr n Hp Pr' PM m k s h STs HPP' Hmn Hkm [HSP HP].
   	  specialize (Hp Pr' HPP' m Hmn HSP).
   	  apply Hp; reflexivity || assumption.
-  	+ intros Pr n Hp Pr' HPP' m Hnm HSP Pr'' PM k l s h t HPP'' Hkm Hkl HP.
+  	+ intros Pr n Hp Pr' HPP' m Hnm HSP Pr'' PM k l s h STs HPP'' Hkm Hkl HP.
   	  apply Hp.
   	  * transitivity Pr'; assumption.
   	  * omega.
